Test/Interpreter/ModArith/encapsulate.mlir
@@ -1,0 +1,11 @@
+// RUN: veir-interpret %s | filecheck %s
+
+"builtin.module"() ({
+  "func.func"() <{sym_name = "main", function_type = () -> !mod_arith.int<251 : i16>}> ({
+    %c243 = "arith.constant"() <{ "value" = 243 : i16 }> : () -> i16
+    %enc = "mod_arith.encapsulate"(%c243) : (i16) -> !mod_arith.int<251 : i16>
+    "func.return"(%enc) : (!mod_arith.int<251 : i16>) -> ()
+  }) : () -> ()
+}) : () -> ()
+
+// CHECK: Program output: #[0x00f3#16]
