Test/ModArith/parity.mlir
@@ -1,0 +1,27 @@
+// RUN: VEIR_ROUNDTRIP
+
+"builtin.module"() ({
+  "func.func"() <{function_type = () -> (), sym_name = "main"}> ({
+    ^bb0():
+      %0 = "mod_arith.constant"() <{"value" = 13 : i32}> : () -> !mod_arith.int<17 : i32>
+      %1 = "mod_arith.extract"(%0) : (!mod_arith.int<17 : i32>) -> i32
+      %2 = "mod_arith.encapsulate"(%1) : (i32) -> !mod_arith.int<17 : i32>
+      %3 = "mod_arith.reduce"(%2) : (!mod_arith.int<17 : i32>) -> !mod_arith.int<17 : i32>
+      %4 = "mod_arith.mac"(%3, %3, %3) : (!mod_arith.int<17 : i32>, !mod_arith.int<17 : i32>, !mod_arith.int<17 : i32>) -> !mod_arith.int<17 : i32>
+      "func.return"() : () -> ()
+  }) : () -> ()
+}) : () -> ()
+
+
+// CHECK:      "builtin.module"() ({
+// CHECK-NEXT:   ^{{.*}}():
+// CHECK-NEXT:     "func.func"() <{"function_type" = () -> (), "sym_name" = "main"}> ({
+// CHECK-NEXT:       ^{{.*}}():
+// CHECK-NEXT:         %{{.*}} = "mod_arith.constant"() <{"value" = 13 : i32}> : () -> !mod_arith.int<17 : i32>
+// CHECK-NEXT:         %{{.*}} = "mod_arith.extract"(%{{.*}}) : (!mod_arith.int<17 : i32>) -> i32
+// CHECK-NEXT:         %{{.*}} = "mod_arith.encapsulate"(%{{.*}}) : (i32) -> !mod_arith.int<17 : i32>
+// CHECK-NEXT:         %{{.*}} = "mod_arith.reduce"(%{{.*}}) : (!mod_arith.int<17 : i32>) -> !mod_arith.int<17 : i32>
+// CHECK-NEXT:         %{{.*}} = "mod_arith.mac"(%{{.*}}, %{{.*}}, %{{.*}}) : (!mod_arith.int<17 : i32>, !mod_arith.int<17 : i32>, !mod_arith.int<17 : i32>) -> !mod_arith.int<17 : i32>
+// CHECK-NEXT:         "func.return"() : () -> ()
+// CHECK-NEXT:     }) : () -> ()
+// CHECK-NEXT: }) : () -> ()
